progress progress

STLC.v
@@ -2,7 +2,8 @@ Set Warnings "-notation-overridden,-parsing".
 Require Import String.
 Require Import Coq.Init.Nat.
 Require Import Coq.Bool.Bool.
-Require Import Coq.Sets.Ensembles.
+Require Import Coq.Lists.ListSet.
+(* Require Import Coq.Sets.Ensembles. *)
 
 (* The Simply-Typed Lambda Calculus *)
 
@@ -72,16 +73,16 @@ Inductive checks (g : gamma) : expr -> ltype -> Prop :=
         checks g e1 (TArrow t t') -> checks g e2 t -> checks g (EApp e1 e2) t'.
 
 (* Free Variables *)
-Fixpoint fv (e : expr) : Ensemble string := 
+Fixpoint fv (e : expr) : set string := 
     match e with
-    | ENat _  => Empty_set string
-    | EBool _ => Empty_set string
-    | EVar x  => Singleton string x
+    | ENat _  => empty_set string
+    | EBool _ => empty_set string
+    | EVar x  => set_add string_dec x (empty_set string)
     | ENot e  => fv e
-    | EBOp _ e1 e2 => Union string (fv e1) (fv e2)
-    | ECond e1 e2 e3 => Union string (Union string (fv e1) (fv e2)) (fv e3)
-    | ELam x _ e => Setminus string (fv e) (Singleton string x)
-    | EApp e1 e2 => Union string (fv e1) (fv e2)
+    | EBOp _ e1 e2 => set_union string_dec (fv e1) (fv e2)
+    | ECond e1 e2 e3 => set_union string_dec (set_union string_dec (fv e1) (fv e2)) (fv e3)
+    | ELam x _ e => set_remove string_dec x (fv e)
+    | EApp e1 e2 => set_union string_dec (fv e1) (fv e2)
     end.
 
 (* Capture-avoiding Substitution *)
@@ -100,11 +101,44 @@ Inductive sub (x : string) (s : expr) : expr -> expr -> Prop :=
         sub x s e1 e1' -> sub x s e2 e2' -> sub x s (EApp e1 e2) (EApp e1' e2')
     | lam_bound_sub : forall (t : ltype) (e : expr),
         sub x s (ELam x t e) (ELam x t e)
-    | lam_free_sub : forall (y : string) (t : ltype) (e e' : expr),
-        x <> y -> not (fv s y) -> sub x s e e' -> sub x s (ELam y t e) (ELam y t e').
+    | lam_notfree_sub : forall (y : string) (t : ltype) (e e' : expr),
+        x <> y -> set_mem string_dec y (fv s) = false -> 
+        sub x s e e' -> sub x s (ELam y t e) (ELam y t e').
+
+Lemma sub_exists : forall (x : string) (s e : expr),
+    exists e', sub x s e e'.
+Proof.
+    intros. induction e.
+    - exists (ENat n). apply natsub.
+    - exists (EBool b). apply boolsub.
+    - destruct (String.eqb x s0) eqn:h.
+        + apply String.eqb_eq in h; subst. exists s.
+            apply hitsub.
+        + rewrite String.eqb_sym in h. 
+            apply String.eqb_neq in h. exists (EVar s0).
+            apply misssub. apply h.
+    - destruct IHe as [e' h]. exists (ENot e').
+        apply notsub. apply h.
+    - destruct IHe1 as [e1' h1]. destruct IHe2 as [e2' h2].
+        exists (EBOp b e1' e2'). apply bopsub.
+        apply h1. apply h2.
+    - destruct IHe1 as [e1' h1]. 
+        destruct IHe2 as [e2' h2]. destruct IHe3 as [e3' h3].
+        exists (ECond e1' e2' e3'). apply condsub.
+        apply h1. apply h2. apply h3.
+    - destruct IHe as [e' h']. destruct (String.eqb x s0) eqn:h.
+        + apply String.eqb_eq in h. subst.
+            exists (ELam s0 l e). apply lam_bound_sub.
+        + rewrite String.eqb_sym in h. 
+            apply String.eqb_neq in h.
+Admitted.
 
 (* Dynamic Semantics *)
 Inductive step : expr -> expr -> Prop :=
+    | notstep : forall (b : bool),
+        step (ENot (EBool b)) (EBool (negb b))
+    | innerstep : forall (e e' : expr),
+        step e e' -> step (ENot e) (ENot e')
     | addstep : forall (n1 n2 : nat),
         step (EBOp EAdd (ENat n1) (ENat n2)) (ENat (n1 + n2))
     | mulstep : forall (n1 n2 : nat),
@@ -119,11 +153,11 @@ Inductive step : expr -> expr -> Prop :=
         step (EBOp EAnd (EBool b1) (EBool b2)) (EBool (andb b1  b2))
     | orstep : forall (b1 b2 : bool),
         step (EBOp EOr (EBool b1) (EBool b2)) (EBool (orb b1  b2))
-    | left_nat_step : forall (op : bop) (n : nat) (e e' : expr),
+    | right_nat_step : forall (op : bop) (n : nat) (e e' : expr),
         step e e' -> step (EBOp op (ENat n) e) (EBOp op (ENat n) e')
-    | left_bool_step : forall (op : bop) (b : bool) (e e' : expr),
+    | right_bool_step : forall (op : bop) (b : bool) (e e' : expr),
         step e e' -> step (EBOp op (EBool b) e) (EBOp op (EBool b) e')
-    | right_bop_step : forall (op : bop) (e1 e1' e2 : expr),
+    | left_bop_step : forall (op : bop) (e1 e1' e2 : expr),
         step e1 e1' -> step (EBOp op e1 e2) (EBOp op e1' e2)
     | truestep : forall (e2 e3 : expr),
         step (ECond (EBool true) e2 e3) e2
@@ -203,12 +237,82 @@ Inductive step : expr -> expr -> Prop :=
             + apply lam_canonical_forms_holds.
     Qed.
         
+    Definition progress (e : expr) (t : ltype) : Prop := 
+        checks empty e t -> value e \/ exists (e' : expr), step e e'.
 
-    Definition preservation (e e' : expr) (t : ltype) : Prop :=
-        step e e' -> checks empty e t -> checks empty e' t.
-
-    Theorem preservation_holds : forall (e e' : expr) (t : ltype),
-        preservation e e' t.
+    Theorem progress_holds : forall (e : expr) (t : ltype), progress e t.
     Proof.
-    Admitted.
+        unfold progress. 
+        induction e; intros.
+        - left. apply natvalue.
+        - left. apply boolvalue.
+        - inversion H. inversion H1.
+        - right. inversion H; subst.
+          apply IHe in H1 as h1. destruct h1 as [h | [e' h]].
+          + apply (bool_canonical_forms_holds e h) in H1 as [b cfh]; subst.
+            exists (EBool (negb b)). apply notstep.
+          + exists (ENot e'). apply innerstep. apply h.
+        - right. inversion H; subst; apply IHe1 in H4 as h1; apply IHe2 in H5 as h2; 
+            destruct h1; destruct h2; 
+            try (apply (nat_canonical_forms_holds e1 H0) in H4 as [n1 v1]; subst;
+            apply (nat_canonical_forms_holds e2 H1) in H5 as [n2 v2]; subst);
+            try (apply (nat_canonical_forms_holds e1 H0) in H4 as [n1 v1]; subst;
+                destruct H1 as [e2' h]);
+            try (apply (bool_canonical_forms_holds e1 H0) in H4 as [b1 v1]; subst;
+            apply (bool_canonical_forms_holds e2 H1) in H5 as [b2 v2]; subst);
+            try (apply (bool_canonical_forms_holds e1 H0) in H4 as [b1 v1]; subst;
+                destruct H1 as [e2' h]);
+            try (destruct H0 as [e1' h]).
+              + exists (ENat (n1 + n2)). apply addstep.
+              + exists (EBOp EAdd (ENat n1) e2'). apply right_nat_step. apply h.
+              + exists (EBOp EAdd e1' e2). apply left_bop_step. apply h.
+              + exists (EBOp EAdd e1' e2). apply left_bop_step. apply h.
+              + exists (ENat (n1 * n2)). apply mulstep.
+              + exists (EBOp EMul (ENat n1) e2'). apply right_nat_step. apply h.
+              + exists (EBOp EMul e1' e2). apply left_bop_step. apply h.
+              + exists (EBOp EMul e1' e2). apply left_bop_step. apply h.
+              + exists (ENat (n1 - n2)). apply substep.
+              + exists (EBOp ESub (ENat n1) e2'). apply right_nat_step. apply h.
+              + exists (EBOp ESub e1' e2). apply left_bop_step. apply h.
+              + exists (EBOp ESub e1' e2). apply left_bop_step. apply h.
+              + exists (EBool (n1 =? n2)). apply eqstep.
+              + exists (EBOp EEq (ENat n1) e2'). apply right_nat_step. apply h.
+              + exists (EBOp EEq e1' e2). apply left_bop_step. apply h.
+              + exists (EBOp EEq e1' e2). apply left_bop_step. apply h.
+              + exists (EBool (n1 <? n2)). apply lestep.
+              + exists (EBOp ELe (ENat n1) e2'). apply right_nat_step. apply h.
+              + exists (EBOp ELe e1' e2). apply left_bop_step. apply h.
+              + exists (EBOp ELe e1' e2). apply left_bop_step. apply h.
+              + exists (EBool (andb b1 b2)). apply andstep.
+              + exists (EBOp EAnd (EBool b1) e2'). apply right_bool_step. apply h.
+              + exists (EBOp EAnd e1' e2). apply left_bop_step. apply h.
+              + exists (EBOp EAnd e1' e2). apply left_bop_step. apply h.
+              + exists (EBool (orb b1 b2)). apply orstep.
+              + exists (EBOp EOr (EBool b1) e2'). apply right_bool_step. apply h.
+              + exists (EBOp EOr e1' e2). apply left_bop_step. apply h.
+              + exists (EBOp EOr e1' e2). apply left_bop_step. apply h.
+        - right. inversion H; subst; 
+          apply IHe1 in H3 as h1; apply IHe2 in H5 as h2; apply IHe3 in H6 as h3; subst.
+          destruct h1 as [h1 | [e1' h1]].
+            + apply (bool_canonical_forms_holds e1 h1) in H3 as [b v1].
+                destruct b; subst.
+                * exists e2. apply truestep.
+                * exists e3. apply falsestep.
+            + exists (ECond e1' e2 e3). apply condstep. apply h1.
+        - left. apply lamvalue.
+        - right. inversion H; subst;
+            apply IHe1 in H2 as h1; apply IHe2 in H4 as h2; subst.
+            destruct h1 as [h1 | [e1' h1]].
+            + apply (lam_canonical_forms_holds e1 t0 t h1) in H2 as [x [e v1]]; subst.
+              assert (hsub: exists e3, sub x e2 e e3).
+ Admitted.
+    
+
+Definition preservation (e e' : expr) (t : ltype) : Prop :=
+    step e e' -> checks empty e t -> checks empty e' t.
+
+Theorem preservation_holds : forall (e e' : expr) (t : ltype),
+    preservation e e' t.
+Proof.
+Admitted.
     
